some more work on ARC, not quite finished with example

ARC.thy
@@ -1,6 +1,6 @@
 theory ARC
 
-imports Main "HOL.Order_Relation"
+imports Main "HOL.Order_Relation" "HOL.Set"
 
 begin
 
@@ -23,21 +23,22 @@ definition wf_model :: "'a pre_model \<Rightarrow> bool"
  (\<forall> n :: noun. f n \<subseteq> U)"
 
 (*The interpretation of a term in a model is a little more complex because we have 
-to handle nouns and complex terms differently*)
+to handle nouns, verbs, and complex terms differently*)
+
+(*hacky workaround for now - ideally some kind of polymorphism would be best here*)
+(*I think it might be better to have this function also handle verbs
+That would require some shenanigans with types because the interpretation 
+of a verb has type 'a x'a set.*)
+fun interp_verb :: "'a pre_model \<Rightarrow> verb \<Rightarrow> ('a \<times> 'a) set" 
+  where "interp_verb M v = (let (U, f, g) = M in (g v))"
+
 fun interp :: "'a pre_model \<Rightarrow> Term \<Rightarrow> 'a set" ("_ interpreting _")
   where 
 "interp M (Noun n) = (let (U, f, g) = M in f n)"
 | "interp M (r all t) = (let (U, f, g) = M in
- {m \<in> U. \<forall> n. (n \<in> (interp M t)) \<longrightarrow> ((m, n) \<in> (g r))})"
+ {m \<in> U. \<forall> n. (n \<in> (interp M t)) \<longrightarrow> ((m, n) \<in> (interp_verb M r))})"
 
 print_theorems
-(*I think it might be better to have this function also handle verbs
-That would require some shenanigans with types because the interpretation 
-of a verb has type 'a x'a set.*)
-
-(*hacky workaround for now - ideally some kind of polymorphism would be best here*)
-fun interp_verb :: "'a pre_model \<Rightarrow> verb \<Rightarrow> ('a \<times> 'a) set" 
-  where "interp_verb M v = (let (U, f, g) = M in (g v))"
 
 fun satisfies :: "'a pre_model \<Rightarrow> sentence \<Rightarrow> bool" ("_ \<Turnstile> _")
   where "satisfies M (All x m) = ((interp M x) \<subseteq> (interp M m))"
@@ -45,22 +46,56 @@ print_theorems
 
 datatype example_universe = e1 | e2 | e3
 
+find_theorems name:satisfies
+
+(*assms(3) was the key to this example. I wasn't able to 
+complete the proof without specifying the universe.*)
 lemma example_model:
   fixes M
   assumes "(UNIV::noun set) = {dog, cat}"
   assumes "(UNIV::verb set) = {see}"
+  assumes "let (U, f, g) = M in (U = (UNIV:: example_universe set))"
   assumes "interp M (Noun dog) = {e2}"
   assumes "interp M (Noun cat) = {e1, e3}"
-  assumes "interp_verb M sees = {(e1, e1), (e1, e2), (e1, e3)}"
-  shows "M \<Turnstile> (All (see all (Noun cat)) (see all (Noun dog)))"
+  assumes "interp_verb M see = {(e2, e1), (e2, e2), (e2, e3)}"
+  assumes "wf_model M"
+  shows "M \<Turnstile> (All (Noun dog) (see all (Noun dog)))"
+and "M \<Turnstile> All (see all (Noun cat)) (see all (Noun dog))"
+proof - 
+  have "{e2} \<subseteq> interp M (see all (Noun dog))" 
+    using assms by force
+  thus "M \<Turnstile> (All (Noun dog) (see all (Noun dog)))"
+    using assms(4) by auto
+  have "interp M (see all (Noun cat)) = {e2}" 
+    using assms by force
+  thus "M \<Turnstile> All (see all (Noun cat)) (see all (Noun dog))"
+    using \<open>{e2} \<subseteq> interp M (see all( Noun dog))\<close> by auto
+qed
 
+definition M_satisfies_G :: "'a pre_model \<Rightarrow> sentence set \<Rightarrow> bool"
+  where "M_satisfies_G M G \<equiv> \<forall> g. g \<in> G \<longrightarrow> satisfies M g"
 
+definition entails :: "sentence set \<Rightarrow> sentence \<Rightarrow> 'a itself \<Rightarrow> bool"
+  where "entails G phi (ty:: 'a itself) \<equiv> \<forall> (M :: 'a pre_model). M_satisfies_G M G \<and> (wf_model M) \<longrightarrow> satisfies M phi"
 
-
-
-
-
-
-
-
-
+find_theorems name:subset_
+lemma example_2_6:
+  shows "entails {All d (chase all a), All c a} (All d (chase all c)) (TYPE(sentence))"
+  unfolding entails_def
+proof (rule+)
+  fix M assume "M_satisfies_G M {All d (chase all a), All c a}"
+  have "M \<Turnstile> All d (chase all a)"
+    by (meson M_satisfies_G_def \<open>M_satisfies_G M {All d (chase all a), All c a}\<close> insertI1)
+  have "M \<Turnstile> All c a"
+    by (meson M_satisfies_G_def \<open>M_satisfies_G M {All d (chase all a), All c a}\<close> insert_subset subset_insertI) 
+  (*have "M \<Turnstile> All d (chase all c)"*)
+  have "M \<Turnstile> All d (chase all c)"
+    unfolding satisfies.simps 
+  proof - 
+    fix x assume "x = interp M d"
+    fix y assume "y = interp M (chase all c)"
+    have "interp M c \<subseteq> interp M a"
+      using \<open>M \<Turnstile> All c a\<close> by auto 
+    then have  "interp M (chase all c) \<subseteq> interp M (chase all a)"
+      unfolding interp.simps using subset_eq  
+  
